veric/res_predicates.v
@@ -701,14 +701,14 @@ Definition LKspec (R: pred rmap) : spec :=
 Definition boolT : Type := bool.
 Definition unitT : Type := unit.
 
-Definition packPQ {A: Type} (P Q: A -> arguments -> pred rmap) := 
-  (fun xy : (A*(boolT*(arguments * unitT))) => 
+Definition packPQ {A: Type} (P Q: A -> list val -> pred rmap) := 
+  (fun xy : (A*(boolT*(list val * unitT))) => 
     if fst (snd xy) then P (fst xy) (fst (snd (snd xy))) else Q (fst xy) (fst (snd (snd xy)))).
 
 Definition TTat (l: address) : pred rmap := TT.
 
-Definition FUNspec (fml: funsig) (A: Type) (P Q: A -> arguments -> pred rmap)(l: address): pred rmap :=
-          allp (jam (eq_dec l) (pureat (SomeP (A::boolT::arguments::nil) (packPQ P Q)) (FUN fml)) TTat).
+Definition FUNspec (fml: funsig) (A: Type) (P Q: A -> list val -> pred rmap)(l: address): pred rmap :=
+          allp (jam (eq_dec l) (pureat (SomeP (A::boolT::list val::nil) (packPQ P Q)) (FUN fml)) TTat).
 
 (***********)
 
@@ -786,10 +786,10 @@ subst; auto.
 Qed.
 
 Lemma FUNspec_parametric: forall fml A P Q, 
-   spec_parametric (fun l sh => yesat (SomeP (A::boolT::arguments::nil) (packPQ P Q)) (FUN fml) sh).
+   spec_parametric (fun l sh => yesat (SomeP (A::boolT::list val::nil) (packPQ P Q)) (FUN fml) sh).
 Proof.
 intros.
-exists (SomeP (A::boolT::arguments::nil) (packPQ P Q)).
+exists (SomeP (A::boolT::list val::nil) (packPQ P Q)).
 exists (fun k => k=FUN fml).
 intros.
 simpl.
@@ -909,7 +909,7 @@ Qed.
 Definition val2address (v: val) : option AV.address := 
   match v with Vptr b ofs => Some (b, Int.signed ofs) | _ => None end.
 
-Definition fun_assert  (v: val) (fml: funsig) (A: Type) (P Q: A -> arguments -> pred rmap) : pred rmap :=
+Definition fun_assert  (v: val) (fml: funsig) (A: Type) (P Q: A -> list val -> pred rmap) : pred rmap :=
  (Ex b : block, !! (v = Vptr b Int.zero) && FUNspec fml A P Q (b,0))%pred.
 
 Definition LK_at l w := exists n, kind_at (LK n) l w.
@@ -1272,15 +1272,15 @@ Qed.
 
 
 Lemma fun_assert_contractive:
-   forall v fml A (P Q: pred rmap -> A -> arguments -> pred rmap), 
+   forall v fml A (P Q: pred rmap -> A -> list val -> pred rmap), 
        (forall x vl, nonexpansive (fun R => P R x vl)) ->
       (forall x vl, nonexpansive (fun R => Q R x vl)) ->
       contractive (fun R : pred rmap => fun_assert v fml A (P R) (Q R)).
 Proof.
 intros.
-assert (H': forall xvl: A * arguments, nonexpansive (fun R => P R (fst xvl) (snd xvl)))
+assert (H': forall xvl: A * list val, nonexpansive (fun R => P R (fst xvl) (snd xvl)))
   by auto; clear H; rename H' into H.
-assert (H': forall xvl: A * arguments, nonexpansive (fun R => Q R (fst xvl) (snd xvl)))
+assert (H': forall xvl: A * list val, nonexpansive (fun R => Q R (fst xvl) (snd xvl)))
   by auto; clear H0; rename H' into H0.
 intro; intros.
 rename H0 into H'.
@@ -1408,19 +1408,6 @@ rewrite H; auto.
 destruct loc; split; unfold adr_add; auto.
 simpl. omega.
 Qed.
-
-(*
-Lemma address_mapsto_core_load:
-  forall ch v sh loc m, 
-    address_mapsto ch v sh loc m -> core_load ch loc v m.
-Proof.
-intros.
-destruct H.
-subst.
-apply core_load_chunk.
-eapply VALspec_range_bytes_readable; eauto.
-Qed.
-*)
 
 Lemma yesat_join_sub:
   forall pp k l rsh sh m m',
